---
layout: article
mathjax: true
title: Proofs of Equivalence
image: "/assets/images/img_test.jpg"
categories:
- DM
desc: To prove a [[Biconditional]] statement $p \leftrightarrow  q$ we have to prove that both statements $p \to q$ and $q \to p$ are true.
 
imagealt: Photo by <a href="https://unsplash.com/@mangofantasy?utm_source=unsplash&utm_medium=referral&utm_content=creditCopyText">Tim Johnson</a> on <a href="https://unsplash.com/s/photos/logic?utm_source=unsplash&utm_medium=referral&utm_content=creditCopyText">Unsplash</a>
---
To prove a [[Biconditional]] statement $p \leftrightarrow  q$ we have to prove that both statements $p \to q$ and $q \to p$ are true.
$$p \leftrightarrow q \to (p \to q ) \wedge (q \to p)$$