---
layout: article
mathjax: true
title: Proofs by Contraposition
image: "/assets/images/img_test.jpg"
categories:
- DM
desc: '' 
imagealt: Photo by <a href="https://unsplash.com/@mangofantasy?utm_source=unsplash&utm_medium=referral&utm_content=creditCopyText">Tim Johnson</a> on <a href="https://unsplash.com/s/photos/logic?utm_source=unsplash&utm_medium=referral&utm_content=creditCopyText">Unsplash</a>
---

[Contrapositive]({% post_url 2020-01-13-contrapositive %}) of [Conditional Statement]({% post_url 2020-01-15-conditional-statement %}) $p \to q$ will be [Equivalent]({% post_url 2020-01-12-equivalent %}) to original statement. So proving the contrapositive ($\neg q \to \neg p$) will also prove original conditional statement.

* We assume the original statement is false, this is our new statement.
* Then we reach [Negation]({% post_url 2020-01-05-negation %}) of [[Conclusion]] (in new statement).
* This proves that [[Hypothesis]] was also false (in new statement.
* Thus, original statement was true.

### Subtopics
- [Vacuous Proofs]({% post_url 2020-04-06-vacuous-proofs %})
- [Trivial Proofs]({% post_url 2020-04-08-trivial-proofs %})