---
layout: article
mathjax: true
title: Inverse of Functions
image: "/assets/images/img_test.jpg"
categories:
- DM
desc: Let $f$ be a [[Bijection]] from $A$ to $B$.
 
imagealt: Photo by <a href="https://unsplash.com/@mangofantasy?utm_source=unsplash&utm_medium=referral&utm_content=creditCopyText">Tim Johnson</a> on <a href="https://unsplash.com/s/photos/logic?utm_source=unsplash&utm_medium=referral&utm_content=creditCopyText">Unsplash</a>
---
Let $f$ be a [[Bijection]] from $A$ to $B$.
*Inverse* of function $f$ assigns an element $b \in B$ to another element $a \in A$ such that $f(a) = b$. Hence, $f^{-1}(b) = a$.

![[Pasted image 20210607124058.png]]