---
layout: article
mathjax: true
title: Strong Induction
image: "/assets/images/img_test.jpg"
categories:
- DM
desc: '' 
imagealt: Photo by <a href="https://unsplash.com/@mangofantasy?utm_source=unsplash&utm_medium=referral&utm_content=creditCopyText">Tim Johnson</a> on <a href="https://unsplash.com/s/photos/logic?utm_source=unsplash&utm_medium=referral&utm_content=creditCopyText">Unsplash</a>
---

The basis step of *Strong Induction* is same as [Principle of Mathematical Induction]({% post_url 2020-08-30-principle-of-mathematical-induction %}) but for *inductive hypothesis* we assume that $P(j)$ is true for all $j = 1, 2, \dots k$.

Induction Step: $[P(1) \wedge P(2) \wedge \dots P(k)] \to P(k+1)$ where $P(n)$ is a [Propositional Function]({% post_url 2020-02-14-propositional-function %}).

It is also known as *Second Principle of Mathematical Induction* or *Complete Induction*.