---
layout: article
mathjax: true
title: Proofs of Equivalence
image: "/assets/images/covers/tim-johnson-Vwf8q3RzBRE-unsplash.jpg"
categories:
- DM
desc: To prove a Biconditional statement $p \leftrightarrow  q$ we have to prove that both statements $p \to q$ and $q \to p$ are true. 
imagealt: Cover Image for article
---

To prove a [Biconditional]({% post_url 2021-06-03-biconditional %}) statement $p \leftrightarrow  q$ we have to prove that both statements $p \to q$ and $q \to p$ are true.




















































































































































































































































































































































































































$$p \leftrightarrow q \to (p \to q ) \wedge (q \to p)$$





















































































































































































































































































































































































































This blog was published directly from my notes.
To check the source of my notes and images used in this blog, visit <a href="/credits.html" target="_blank">Credits</a>.

To read my notes, download this <a href="https://github.com/bovem/CS" target="blank">repository</a>.