---
layout: article
mathjax: true
title: Multiplication of Generating Functions
image: "/assets/images/covers/tim-johnson-Vwf8q3RzBRE-unsplash.jpg"
categories:
- DM
desc: $f(x) = \sum_{k=0}^{ \infty } a_k x^k$ and $g(x) = \sum_{k=0}^{ \infty } b_k x^k$. 
imagealt: Cover Image for article
---

$f(x) = \sum_{k=0}^{ \infty } a_k x^k$ and $g(x) = \sum_{k=0}^{ \infty } b_k x^k$.




















































































































































































































































































































































































































Then
$$f(x)g(x) = \sum_{k=0}^{\infty} \ (\sum_{j=0}^{ k } (a_j b_{k-j}))\ x^k$$





















































































































































































































































































































































































































This blog was published directly from my notes.
To check the source of my notes and images used in this blog, visit <a href="/credits.html" target="_blank">Credits</a>.

To read my notes, download this <a href="https://github.com/bovem/CS" target="blank">repository</a>.